src/Wf.v
@@ -1,0 +1,90 @@
+Require Import Bool List String Structures.Equalities.
+Require Import Lib.Struct Lib.Word Lib.CommonTactics Lib.StringBound Lib.ilist Lib.FnMap.
+Require Import Syntax.
+Require Import FunctionalExtensionality Program.Equality Eqdep Eqdep_dec.
+
+Set Implicit Arguments.
+
+(* Well-formedness w.r.t. structural hazards:
+ * 1) No double-writes and 2) No double-calls for all actions in Modules
+ *)
+Section Wf1.
+  Variable type: Kind -> Type.
+
+  Fixpoint appendAction {retT1 retT2} (a1: ActionT type retT1)
+           (a2: type retT1 -> ActionT type retT2): ActionT type retT2 :=
+    match a1 with
+      | MCall name sig ar cont => MCall name sig ar (fun a => appendAction (cont a) a2)
+      | Let_ _ ar cont => Let_ ar (fun a => appendAction (cont a) a2)
+      | ReadReg reg k cont => ReadReg reg k (fun a => appendAction (cont a) a2)
+      | WriteReg reg _ e cont => WriteReg reg e (appendAction cont a2)
+      | IfElse ce _ ta fa cont => IfElse ce ta fa (fun a => appendAction (cont a) a2)
+      | Assert_ ae cont => Assert_ ae (appendAction cont a2)
+      | Return e => Let_ e a2
+    end.
+
+  Lemma appendAction_assoc:
+    forall {retT1 retT2 retT3}
+           (a1: ActionT type retT1) (a2: type retT1 -> ActionT type retT2)
+           (a3: type retT2 -> ActionT type retT3),
+      appendAction a1 (fun t => appendAction (a2 t) a3) = appendAction (appendAction a1 a2) a3.
+  Proof.
+    induction a1; simpl; intuition idtac; f_equal; try extensionality x; eauto.
+  Qed.
+
+  Inductive WfAction: list string -> list string -> forall {retT}, ActionT type retT -> Prop :=
+  | WfMCall:
+      forall regs calls name sig ar {retT} cont (Hnin: ~ In name calls),
+        (forall t, WfAction regs (name :: calls) (cont t)) ->
+        WfAction regs calls (MCall (lretT:= retT) name sig ar cont)
+  | WfLet:
+      forall regs calls {argT retT} ar cont,
+        (forall t, WfAction regs calls (cont t)) ->
+        WfAction regs calls (Let_ (lretT':= argT) (lretT:= retT) ar cont)
+  | WfReadReg:
+      forall regs calls {retT} reg k cont,
+        (forall t, WfAction regs calls (cont t)) ->
+        WfAction regs calls (ReadReg (lretT:= retT) reg k cont)
+  | WfWriteReg:
+      forall regs calls {writeT retT} reg e cont (Hnin: ~ In reg regs),
+        WfAction regs calls cont ->
+        WfAction (reg :: regs) calls (WriteReg (k:= writeT) (lretT:= retT) reg e cont)
+  | WfIfElse:
+      forall regs calls {retT1 retT2} ce ta fa cont,
+        WfAction regs calls (appendAction (retT1:= retT1) (retT2:= retT2) ta cont) ->
+        WfAction regs calls (appendAction (retT1:= retT1) (retT2:= retT2) fa cont) ->
+        WfAction regs calls (IfElse ce ta fa cont)
+  | WfAssert:
+      forall regs calls {retT} e cont,
+        WfAction regs calls cont ->
+        WfAction regs calls (Assert_ (lretT:= retT) e cont)
+  | WfReturn:
+      forall regs calls {retT} (e: Expr type (SyntaxKind retT)), WfAction regs calls (Return e).
+
+  Inductive WfRules: list (Attribute (Action Void)) -> Prop :=
+  | WfRulesNil: WfRules nil
+  | WfRulesCons:
+      forall rule rules,
+        WfRules rules ->
+        WfAction nil nil ((attrType rule) type) ->
+        WfRules (rule :: rules).
+
+  Inductive WfDms: list DefMethT -> Prop :=
+  | WfDmsNil: WfDms nil
+  | WfDmsCons:
+      forall (dm: DefMethT) dms,
+        WfDms dms ->
+        (forall argV, WfAction nil nil (objVal (attrType dm) type argV)) ->
+        WfDms (dm :: dms).
+
+  Inductive WfModules: Modules -> Prop :=
+  | WfMod:
+      forall regs rules dms,
+        WfRules rules -> WfDms dms -> WfModules (Mod regs rules dms)
+  | WfConcatMod:
+      forall m1 m2,
+        WfModules m1 -> WfModules m2 -> WfModules (ConcatMod m1 m2).
+
+End Wf1.
+
+
